\sbs{\small Приёмы интегрирования}

\begin{minipage}[t]{0.45\textwidth}
%%%%%%%%%%%%%%%%%%%%%%%%%%%%%%%%%%%%%%%%%%%%%%%%%%%%%%%%%%%%%%%%%%%%%%%%
\begin{proof}[
thr $\triangle$
\eqref{4.121}]

\phantom{42}

\noindent
1) $F = fg$ -- непр на $[a, b]$ и дифф на $(a, b)$. \\
$F' = f'g + f g'$ $\in \mathcal R$ как $\int \cdot$. 
\end{proof}
%%%%%%%%%%%%%%%%%%%%%%%%%%%%%%%%%%%%%%%%%%%%%%%%%%%%%%%%%%%%%%%%%%%%%%%%
\end{minipage}
\hfill
\begin{minipage}[t]{0.45\textwidth}
%%%%%%%%%%%%%%%%%%%%%%%%%%%%%%%%%%%%%%%%%%%%%%%%%%%%%%%%%%%%%%%%%%%%%%%%
\begin{proof}[
thr $\triangle$
\eqref{4.122}]

\phantom{42}

\noindent
1) Если $F' = f$, то $\lr{F(\varphi)}'=f(\varphi) \varphi'$. \\
2) всё непр. $\Rightarrow$ по Н-Л ...
\end{proof}
%%%%%%%%%%%%%%%%%%%%%%%%%%%%%%%%%%%%%%%%%%%%%%%%%%%%%%%%%%%%%%%%%%%%%%%%
\end{minipage}

\phantom{42}

\begin{minipage}[t]{0.9\textwidth}
%%%%%%%%%%%%%%%%%%%%%%%%%%%%%%%%%%%%%%%%%%%%%%%%%%%%%%%%%%%%%%%%%%%%%%%%
\begin{proof}[
thr $\triangle$
\eqref{4.123}]

\phantom{42}

\noindent
1) $n=1$: $f(x) = f(x_0) + \int_{x_0}^{x} f' \d t$. \\
2) $\int_{x_0}^x \frac{f^{(n)} (t)}{(n-1)!} (x-t)^{n-1} \d t = 
- \int_{x_0}^{x} \frac{f^{(n)}(t)}{(n-1)!} \d \frac{(x-t)^n}{n} 
=- \int_{x_0}^{x} \frac{f^{(n)}(t)}{n!} \d (x-t)^n =$ \\
$= - \frac{f^{(n)}(t)}{n!} (x-t)^n \big|_{x_0}^x + \int_{x_0}^x \frac{f^{(n+1)}(t)}{n!} (x-t)^n \d t = - \frac{f^{(n)}(t)}{n!} (x-x_0)^n + \int_{x_0}^x \frac{f^{(n+1)}(t)}{n!} (x-t)^n \d t$.
\end{proof}
%%%%%%%%%%%%%%%%%%%%%%%%%%%%%%%%%%%%%%%%%%%%%%%%%%%%%%%%%%%%%%%%%%%%%%%%
\end{minipage}